feat(SR): Updated checker with FFI-backed parser

Experiments/SR/Data/ByteArray/FFI/byte_array_ffi_defs.c
@@ -1,0 +1,184 @@
+#include <ctype.h>
+#include <stdio.h>
+#include <lean/lean.h>
+
+size_t lean_byte_array_ws(lean_object* arr, size_t iter) {
+  size_t arr_size = lean_sarray_size(arr);
+  for (; iter < arr_size; iter++) {
+    uint8_t ch = lean_byte_array_uget(arr, iter);
+    if (!isspace(ch)) {
+      break;
+    }
+  }
+
+  return iter; 
+}
+
+size_t lean_byte_array_line(lean_object* arr, size_t iter) {
+  size_t arr_size = lean_sarray_size(arr);
+  for (; iter < arr_size; iter++) {
+    uint8_t ch = lean_byte_array_uget(arr, iter);
+    if (ch == '\n') {
+      return iter + 1;
+    }
+  }
+
+  return iter;
+}
+
+size_t lean_byte_array_token(lean_object*arr, size_t iter) {
+  size_t arr_size = lean_sarray_size(arr);
+  for (; iter < arr_size; iter++) {
+    uint8_t ch = lean_byte_array_uget(arr, iter);
+    if (!isspace(ch)) {
+      break;
+    }
+  }
+
+  for (; iter < arr_size; iter++) {
+    uint8_t ch = lean_byte_array_uget(arr, iter);
+    if (isspace(ch)) {
+      break;
+    }
+  }
+
+  return iter;
+}
+
+size_t lean_byte_array_skip_nat_no_ws(lean_object* arr, size_t iter) {
+  size_t arr_size = lean_sarray_size(arr);
+  for (; iter < arr_size; iter++) {
+    uint8_t ch = lean_byte_array_uget(arr, iter);
+    if (!isdigit(ch)) {
+      break; 
+    }
+  }
+
+  return iter; 
+}
+
+size_t lean_byte_array_skip_int_no_ws(lean_object* arr, size_t iter) {
+  size_t arr_size = lean_sarray_size(arr);
+  if (iter < arr_size) {
+    uint8_t ch = lean_byte_array_uget(arr, iter);
+    if (ch == '-') {
+      iter++;
+    }
+  }
+
+  return lean_byte_array_skip_nat_no_ws(arr, iter);
+}
+
+////////////////////////////////////////////////////////////////////////////////
+// readNat, readInt
+////////////////////////////////////////////////////////////////////////////////
+
+static lean_obj_res lean_byte_array_read_panic_oob(lean_obj_arg def_val) {
+  return lean_panic_fn(def_val, lean_mk_ascii_string_unchecked(
+    "Attempted to read a number, but the iterator is out of bounds."));
+}
+
+static lean_obj_res lean_byte_array_read_panic_nan(lean_obj_arg def_val) {
+  return lean_panic_fn(def_val, lean_mk_ascii_string_unchecked(
+    "Attempted to read a number, but the first non-whitespace character is not a digit or '-': "));
+}
+
+uint32_t lean_byte_array_read_uint32_no_ws(lean_object* arr, size_t iter) {
+  size_t arr_size = lean_sarray_size(arr);
+  if (iter < arr_size) {
+    uint8_t ch = lean_byte_array_uget(arr, iter);
+    if (!isdigit(ch)) {
+      lean_byte_array_read_panic_nan(lean_box_uint32((uint32_t) ch));
+    }
+
+    uint32_t acc = 0;
+    for (; iter < arr_size; iter++) {
+      ch = lean_byte_array_uget(arr, iter);
+      if (!isdigit(ch)) {
+        break;
+      }
+
+      acc = acc * 10 + ((uint32_t) (ch - '0'));
+    }
+
+    return acc;
+  } else {
+    lean_byte_array_read_panic_oob(lean_box_usize(iter));
+    return 0; // Unreachable
+  }
+}
+
+lean_object* lean_byte_array_read_int32_no_ws(lean_object* arr, size_t iter) {
+  size_t arr_size = lean_sarray_size(arr);
+  if (iter < arr_size) {
+    uint8_t ch = lean_byte_array_uget(arr, iter);
+
+    // Handle a starting minus sign
+    int starts_with_minus = 0;
+    if (ch == '-') {
+      iter++;
+      starts_with_minus = 1;
+    }
+    
+    int32_t acc = (int32_t) lean_byte_array_read_uint32_no_ws(arr, iter);
+
+    if (starts_with_minus) {
+      acc = -acc;
+    }
+
+    return lean_int32_to_int((uint32_t) acc);
+  } else {
+    lean_byte_array_read_panic_oob(lean_box_usize(iter));
+    return NULL; // Unreachable
+  }
+}
+
+uint64_t lean_byte_array_read_uint64_no_ws(lean_object* arr, size_t iter) {
+  size_t arr_size = lean_sarray_size(arr);
+  if (iter < arr_size) {
+    uint8_t ch = lean_byte_array_uget(arr, iter);
+    if (!isdigit(ch)) {
+      lean_byte_array_read_panic_nan(lean_box_uint32((uint32_t) ch));
+    }
+
+    uint64_t acc = 0;
+    for (; iter < arr_size; iter++) {
+      ch = lean_byte_array_uget(arr, iter);
+      if (!isdigit(ch)) {
+        break;
+      }
+
+      acc = acc * 10 + ((uint64_t) (ch - '0'));
+    }
+
+    return acc;
+  } else {
+    lean_byte_array_read_panic_oob(lean_box_usize(iter));
+    return 0; // Unreachable
+  }
+}
+
+lean_object* lean_byte_array_read_int64_no_ws(lean_object* arr, size_t iter) {
+  size_t arr_size = lean_sarray_size(arr);
+  if (iter < arr_size) {
+    uint8_t ch = lean_byte_array_uget(arr, iter);
+
+    // Handle a starting minus sign
+    int starts_with_minus = 0;
+    if (ch == '-') {
+      iter++;
+      starts_with_minus = 1;
+    }
+    
+    int64_t acc = (int64_t) lean_byte_array_read_uint64_no_ws(arr, iter);
+
+    if (starts_with_minus) {
+      acc = -acc;
+    }
+
+    return lean_int64_to_int((uint64_t) acc);
+  } else {
+    lean_byte_array_read_panic_oob(lean_box_usize(iter));
+    return NULL; // Unreachable
+  }
+}
