Experiments/SR/Data/UInt/FFI/uint_ffi_defs.c
@@ -1,0 +1,19 @@
+#include <ctype.h>
+#include <stdio.h>
+#include <lean/lean.h>
+
+bool uint8_is_digit(uint8_t ch) {
+  return isdigit(ch);
+}
+
+bool uint8_is_space(uint8_t ch) {
+  return isspace(ch);
+}
+
+bool uint32_is_digit(uint32_t ch) {
+  return isdigit(ch);
+}
+
+bool uint32_is_space(uint32_t ch) {
+  return isspace(ch);
+}
