Experiments/SR/Data/ByteArray/Basic.lean
@@ -1,0 +1,614 @@
+
+import Lean
+import Experiments.SR.Data.ByteArray.Defs
+
+open Lean
+open Lean.Elab
+open Lean.Elab.Tactic
+
+/-- A common sequence of tactics for proving termination of an iterator
+    getting closer to the size of an array. Via `USize.sub_succ_lt_sub_of_lt`. -/
+macro "sub_succ" : tactic => `(tactic| (
+    simp
+    apply USize.lt_iff_toNat_lt.mp
+    apply USize.sub_succ_lt_sub_of_lt
+    assumption
+  ))
+
+namespace ByteArray
+
+/-! # peek -/
+
+theorem iter_lt_of_peek_ne_EOF {arr : ByteArray} {iter : USize}
+    : peek arr iter ≠ UInt8.EOF → iter < arr.size.toUSize := by
+  unfold peek
+  simp
+  exact fun hi _ => hi
+
+theorem peek_eq_of_ge_size {arr : ByteArray} {iter : USize}
+    : iter ≥ arr.size.toUSize → peek arr iter = UInt8.EOF := by
+  unfold peek
+  simp
+  intro h h_con
+  exact absurd h (USize.not_le.mpr h_con)
+
+@[simp]
+theorem peek_eq_size (arr : ByteArray) : peek arr arr.size.toUSize = UInt8.EOF :=
+  peek_eq_of_ge_size (USize.le_refl _)
+
+/-! # skip -/
+
+@[simp]
+theorem iter_le_skip (arr : ByteArray) (iter : USize) (pred : UInt8 → Bool)
+    : iter ≤ skip arr iter pred := by
+  unfold skip
+  simp
+  split
+  · rename_i hi
+    split
+    · have := iter_le_skip arr (iter + 1) pred
+      apply USize.le_trans (USize.le_of_lt _) this
+      exact USize.lt_succ_of_lt hi
+    · apply Nat.le_refl
+  · apply Nat.le_refl
+termination_by arr.size.toUSize - iter
+decreasing_by sub_succ
+
+theorem iter_lt_skip_of_peek_ne_EOF_of_pred_true {arr : ByteArray} {iter : USize} {pred : UInt8 → Bool}
+    : peek arr iter ≠ UInt8.EOF → pred (peek arr iter) → iter < skip arr iter pred := by
+  unfold skip
+  simp
+  split
+  <;> rename_i hi
+  · intro h_peek h_pred
+    simp [peek, hi] at h_pred
+    simp [h_pred]
+    apply USize.lt_of_lt_of_le <| USize.lt_succ_of_lt hi
+    apply iter_le_skip
+  · simp [peek_eq_of_ge_size (USize.not_lt.mp hi)]
+
+theorem iter_lt_skip_of_pred_uget_true {arr : ByteArray} {iter : USize} {pred : UInt8 → Bool}
+      {hi : iter < arr.size.toUSize}
+    : pred (arr.uget iter (USize.toNat_lt_of_lt_toUSize hi)) → iter < skip arr iter pred := by
+  unfold skip
+  simp [hi]
+  intro hp
+  simp [hp]
+  apply USize.lt_of_lt_of_le <| USize.lt_succ_of_lt hi
+  apply iter_le_skip
+
+theorem skip_eq_of_peek_pred_false {arr : ByteArray} {iter : USize} {pred : UInt8 → Bool}
+    : ¬pred (peek arr iter) → skip arr iter pred = iter := by
+  unfold skip peek
+  simp
+  intro hp hi hp'
+  simp [hi, hp'] at hp
+
+theorem skip_eq_of_uget_pred_false {arr : ByteArray} {iter : USize} {pred : UInt8 → Bool}
+    (hi : iter < arr.size.toUSize)
+    : ¬pred (arr.uget iter (USize.toNat_lt_of_lt_toUSize hi)) → skip arr iter pred = iter := by
+  unfold skip
+  simp [hi]
+  intro hp hp'
+  simp [hp'] at hp
+
+theorem skip_eq_of_ge_size {arr : ByteArray} {iter : USize}
+    : iter ≥ arr.size.toUSize → ∀ pred, skip arr iter pred = iter := by
+  intro hi pred
+  unfold skip
+  simp [USize.not_lt.mpr hi]
+
+@[simp]
+theorem skip_eq_size (arr : ByteArray) (pred : UInt8 → Bool)
+    : skip arr arr.size.toUSize pred = arr.size.toUSize := by
+  apply skip_eq_of_ge_size
+  exact USize.le_refl _
+
+theorem skip_le_of_le {arr : ByteArray} {iter : USize}
+    : iter ≤ arr.size.toUSize → ∀ pred, skip arr iter pred ≤ arr.size.toUSize := by
+  intro hi pred
+  rcases USize.lt_or_eq_of_le hi with (h | rfl)
+  · unfold skip
+    simp [h]
+    split
+    · exact skip_le_of_le (USize.succ_le_of_lt h) pred
+    · exact hi
+  · simp
+termination_by arr.size.toUSize - iter
+decreasing_by sub_succ
+
+theorem le_skip_of_le {iter₁ iter₂ : USize}
+    : iter₁ ≤ iter₂ → ∀ arr pred, iter₁ ≤ skip arr iter₂ pred := by
+  intro hi arr pred
+  apply USize.le_trans hi
+  exact iter_le_skip arr iter₂ pred
+
+@[simp]
+theorem skip_skip (arr : ByteArray) (iter : USize) (pred : UInt8 → Bool)
+    : skip arr (skip arr iter pred) pred = skip arr iter pred := by
+  unfold skip
+  stop
+  simp
+  split
+  · rename_i hsi
+    split
+    · split
+      · split
+        ·
+          done
+        done
+      done
+    done
+  ·
+    done
+  done
+
+
+/-! # ws -/
+
+@[simp]
+theorem iter_le_ws (arr : ByteArray) (iter : USize) : iter ≤ ws arr iter :=
+  iter_le_skip arr iter _
+
+theorem ws_eq_of_ge_size {arr : ByteArray} {iter : USize}
+    : iter ≥ arr.size.toUSize → ws arr iter = iter := by
+  unfold ws
+  intro hi
+  apply skip_eq_of_ge_size hi
+
+@[simp]
+theorem ws_eq_size (arr : ByteArray) : ws arr arr.size.toUSize = arr.size.toUSize :=
+  ws_eq_of_ge_size (USize.le_refl _)
+
+theorem ws_le_of_le {arr : ByteArray} {iter : USize}
+    : iter ≤ arr.size.toUSize → ws arr iter ≤ arr.size.toUSize := by
+  intro hi
+  unfold ws
+  apply skip_le_of_le hi
+
+theorem ws_eq_of_peek_isDigit {arr : ByteArray} {iter : USize}
+    : (peek arr iter).isDigit → ws arr iter = iter := by
+  intro h
+  unfold ws
+  apply skip_eq_of_peek_pred_false
+  exact UInt8.not_isSpace_of_isDigit h
+
+theorem ws_eq_of_uget_isDigit {arr : ByteArray} {iter : USize} (hi : iter < arr.size.toUSize)
+    : (arr.uget iter (USize.toNat_lt_of_lt_toUSize hi)).isDigit → ws arr iter = iter := by
+  intro h
+  unfold ws
+  apply skip_eq_of_uget_pred_false hi
+  exact UInt8.not_isSpace_of_isDigit h
+
+@[simp]
+theorem ws_ws (arr : ByteArray) (iter : USize) : ws arr (ws arr iter) = ws arr iter :=
+  skip_skip arr iter _
+
+/-! # line -/
+
+@[simp]
+theorem iter_le_line (arr : ByteArray) (iter : USize)
+    : iter ≤ line arr iter := by
+  unfold line
+  simp
+  split
+  · rename_i hi
+    apply USize.le_of_le_of_lt <| iter_le_skip arr iter (! ·.isNewline)
+    apply USize.lt_succ_of_lt hi
+  · simp
+
+theorem line_le_of_le {arr : ByteArray} {iter : USize}
+    : iter ≤ arr.size.toUSize → line arr iter ≤ arr.size.toUSize := by
+  intro hi
+  unfold line
+  simp
+  split
+  · rename_i h
+    apply USize.succ_le_of_lt h
+  · apply skip_le_of_le hi
+
+theorem line_eq_of_ge_size {arr : ByteArray} {iter : USize}
+    : iter ≥ arr.size.toUSize → line arr iter = iter := by
+  intro hi
+  unfold line
+  simp
+  simp [skip_eq_of_ge_size hi, USize.not_lt.mpr hi]
+
+@[simp]
+theorem line_eq_size (arr : ByteArray) : line arr arr.size.toUSize = arr.size.toUSize :=
+  line_eq_of_ge_size (USize.le_refl _)
+
+theorem le_line_of_le (arr : ByteArray) {iter₁ iter₂ : USize}
+    : iter₁ ≤ iter₂ → iter₁ ≤ line arr iter₂ := by
+  intro hi
+  simp [line]
+  split
+  · rename_i hs
+    apply USize.le_trans <| le_skip_of_le hi arr (! ·.isNewline)
+    apply USize.le_of_lt
+    exact USize.lt_succ_of_lt hs
+  · apply le_skip_of_le hi
+
+/-! # token -/
+
+@[simp]
+theorem iter_le_token (arr : ByteArray) (iter : USize)
+    : iter ≤ token arr iter := by
+  unfold token
+  simp
+  apply USize.le_trans <| iter_le_ws arr iter
+  apply iter_le_skip
+
+theorem token_eq_of_ge_size {arr : ByteArray} {iter : USize}
+    : iter ≥ arr.size.toUSize → token arr iter = iter := by
+  intro hi
+  unfold token
+  simp [ws_eq_of_ge_size hi, skip_eq_of_ge_size hi]
+
+@[simp]
+theorem token_eq_size {arr : ByteArray} : token arr arr.size.toUSize = arr.size.toUSize :=
+  token_eq_of_ge_size (USize.le_refl _)
+
+theorem token_le_of_le {arr : ByteArray} {iter : USize}
+    : iter ≤ arr.size.toUSize → token arr iter ≤ arr.size.toUSize := by
+  intro hi
+  unfold token
+  simp
+  apply skip_le_of_le
+  exact ws_le_of_le hi
+
+/-! # skipNat, skipInt -/
+
+@[simp]
+theorem skipNoWs_eq_size (arr : ByteArray)
+    : skipNatNoWs arr arr.size.toUSize = arr.size.toUSize := by
+  unfold skipNatNoWs; simp
+
+theorem skipNatNoWs_le_of_le {arr : ByteArray} {iter : USize}
+    : iter ≤ arr.size.toUSize → skipNatNoWs arr iter ≤ arr.size.toUSize :=
+  fun hi => skip_le_of_le hi fun x => x.isDigit
+
+@[simp]
+theorem le_skipNatNoWs (arr : ByteArray) (iter : USize)
+    : iter ≤ skipNatNoWs arr iter := by
+  unfold skipNatNoWs; simp
+
+theorem iter_lt_skipNatNoWs_of_peek_isDigit {arr : ByteArray} {iter : USize}
+    : UInt8.isDigit (peek arr iter) → iter < skipNatNoWs arr iter := by
+  intro h_peek
+  apply iter_lt_skip_of_peek_ne_EOF_of_pred_true _ h_peek
+  apply UInt8.ne_EOF_of_isDigit h_peek
+
+
+theorem skipInt_le_of_le {arr : ByteArray} {iter : USize}
+    : iter ≤ arr.size.toUSize → skipInt arr iter ≤ arr.size.toUSize := by
+  stop
+  intro hi
+  unfold skipInt
+  simp
+  split
+  · rename_i h_neg
+    apply skip_le_of_le hi fun x => x.isDigit || x == UInt8._minus
+    simp [h_neg]
+  · apply skipNatNoWs_le_of_le hi
+
+/-! # readNat, readInt -/
+
+section readNat
+
+variable {α : Type u} [ParseNumeric α]
+
+@[simp]
+theorem iter_le_readNatNoWs (arr : ByteArray) (iter : USize) (acc : α)
+    : iter ≤ (readNatNoWs (α := α) arr iter acc).2 := by
+  unfold readNatNoWs
+  simp
+  split
+  · rename_i hi
+    split
+    · apply USize.le_of_lt_of_le <| USize.lt_succ_of_lt hi
+      apply iter_le_readNatNoWs
+    · exact USize.le_rfl
+  · simp
+termination_by arr.size.toUSize - iter
+decreasing_by sub_succ
+
+theorem iter_lt_readNatNoWs_of_ne_zero {arr : ByteArray} {iter : USize}
+    : (readNatNoWs (α := α) arr iter).1 ≠ 0 → iter < (readNatNoWs (α := α) arr iter).2 := by
+  unfold readNatNoWs
+  by_cases hi : iter < arr.size.toUSize
+  <;> simp [hi]
+  · intro h
+    split
+    <;> rename_i h_uget
+    <;> simp [h_uget] at h
+    · apply USize.lt_of_lt_of_le <| USize.lt_succ_of_lt hi
+      simp
+
+theorem readNatNoWs_le_of_le {arr : ByteArray} {iter : USize}
+    : iter ≤ arr.size.toUSize → ∀ acc, (readNatNoWs (α := α) arr iter acc).2 ≤ arr.size.toUSize := by
+  intro hi acc
+  unfold readNatNoWs
+  simp
+  split
+  · rename_i hi_lt
+    split
+    · apply readNatNoWs_le_of_le
+      exact USize.succ_le_of_lt hi_lt
+    · exact hi
+  · exact hi
+termination_by arr.size.toUSize - iter
+decreasing_by sub_succ
+
+@[simp]
+theorem iter_le_readNat (arr : ByteArray) (iter : USize)
+    : iter ≤ (readNat (α := α) arr iter).2 := by
+  unfold readNat
+  simp
+  split
+  · apply USize.le_trans <| iter_le_ws arr iter
+    apply iter_le_readNatNoWs
+  · apply iter_le_ws
+
+theorem iter_lt_readNat_of_ne_zero {arr : ByteArray} {iter : USize}
+    : (readNat (α := α) arr iter).1 ≠ 0 → iter < (readNat (α := α) arr iter).2 := by
+  unfold readNat
+  simp
+  split
+  · rename_i h_ws
+    intro h
+    apply USize.lt_of_le_of_lt <| iter_le_ws arr iter
+    exact iter_lt_readNatNoWs_of_ne_zero h
+  · simp
+
+@[simp]
+theorem iter_le_readInt (arr : ByteArray) (iter : USize)
+    : iter ≤ (readInt (α := α) arr iter).2 := by
+  unfold readInt
+  simp
+  split
+  · rename_i hp
+    simp
+    apply USize.le_trans <| iter_le_ws arr iter
+    have : peek arr (ws arr iter) ≠ UInt8.EOF := by simp [hp]; trivial
+    replace := iter_lt_of_peek_ne_EOF this
+    apply USize.le_of_lt_of_le <| USize.lt_succ_of_lt this
+    apply iter_le_readNatNoWs
+  · split
+    · apply USize.le_trans <| iter_le_ws arr iter
+      apply iter_le_readNatNoWs
+    · simp
+
+theorem iter_lt_readInt_iter_of_ne_zero {arr : ByteArray} {iter : USize}
+    : (readInt (α := α) arr iter).1 ≠ 0 → iter < (readInt (α := α) arr iter).2 := by
+  unfold readInt
+  simp
+  split
+  · rename_i hp
+    simp
+    intro h
+    have : peek arr (ws arr iter) ≠ UInt8.EOF := by simp [hp]; trivial
+    replace := iter_lt_of_peek_ne_EOF this
+    apply USize.lt_of_le_of_lt <| iter_le_ws arr iter
+    apply USize.lt_of_lt_of_le <| USize.lt_succ_of_lt this
+    apply iter_le_readNatNoWs
+  · split
+    · simp
+      intro h
+      apply USize.lt_of_le_of_lt <| iter_le_ws arr iter
+      apply iter_lt_readNatNoWs_of_ne_zero
+      intro h_con
+      simp [h_con] at h
+    · simp
+
+theorem iter_lt_skipNat_of_readUInt32NoWs.loop_ne_zero {arr : ByteArray} {iter : USize}
+    : readUInt32NoWs.loop arr iter 0 ≠ 0 → iter < skipNat arr iter := by
+  unfold readUInt32NoWs.loop skipNat skipNatNoWs
+  simp
+  intro hi hd h_nz
+  rw [ws_eq_of_uget_isDigit hi hd]
+  apply iter_lt_skip_of_pred_uget_true hd
+  exact hi
+
+theorem iter_lt_skipNat_of_readUInt32NoWs_ne_zero {arr : ByteArray} {iter : USize}
+    : readUInt32NoWs arr iter ≠ 0 → iter < skipNat arr iter := by
+  unfold readUInt32NoWs
+  simp
+  intro _ _
+  apply iter_lt_skipNat_of_readUInt32NoWs.loop_ne_zero
+
+theorem iter_lt_skipNat_of_readUInt32 {arr : ByteArray} {iter}
+    : readUInt32 arr iter ≠ 0 → iter < skipNat arr iter := by
+  unfold readUInt32 skipNat
+  simp
+  intro h
+  apply USize.lt_of_le_of_lt <| iter_le_ws arr iter
+  have := iter_lt_skipNat_of_readUInt32NoWs_ne_zero h
+  simp [skipNat] at this
+  exact this
+
+theorem iter_lt_skipInt_of_readInt32NoWs {arr : ByteArray} {iter : USize}
+    : readInt32NoWs arr iter ≠ 0 → iter < skipInt arr iter := by
+  unfold readInt32NoWs skipInt
+  simp
+  intro hi h
+  stop
+  split at h
+  · simp at h
+    done
+  ·
+    done
+  rw [ws_eq_of_uget_isDigit hi h_neg]
+  apply iter_lt_skip_of_pred_uget_true h_neg
+  exact hi
+
+theorem iter_lt_skipInt_of_readInt32 {arr : ByteArray} {iter}
+    : readInt32 arr iter ≠ 0 → iter < skipInt arr iter := by
+  unfold readInt32 skipInt
+  stop
+  simp
+  intro h
+  apply USize.lt_of_le_of_lt <| iter_le_ws arr iter
+  have := iter_lt_skipNat_of_readUInt32NoWs_ne_zero h
+  simp [skipInt, skipNat] at this
+  exact this
+
+
+end readNat
+
+#exit
+@[simp]
+private theorem iter_le_readNatNoWs_loop (arr : ByteArray) (iter : USize) (acc : α)
+    : iter ≤ (readNatNoWs.loop arr iter acc).2 := by
+  unfold readNatNoWs.loop
+  simp
+  split
+  · rename_i hi
+    split
+    · apply USize.le_of_lt_of_le (USize.lt_succ_of_lt hi)
+      apply iter_le_readNatNoWs_loop
+    · split
+      · apply USize.le_refl
+      · exact USize.le_of_lt hi
+  · exact Nat.le_refl _
+termination_by arr.size.toUSize - iter
+decreasing_by simp; apply USize.lt_iff_toNat_lt.mp; apply USize.sub_succ_lt_sub_of_lt; assumption
+
+@[simp]
+theorem iter_le_readNatNoWs (arr : ByteArray) (iter : USize)
+    : iter ≤ (readNatNoWs (α := α) arr iter).2 := by
+  unfold readNatNoWs; simp; split <;> simp
+
+@[simp]
+private theorem readNatNoWs_loop_eq (arr : ByteArray) (acc : α)
+    : readNatNoWs.loop arr arr.size.toUSize acc = (acc, arr.size.toUSize) := by
+  unfold readNatNoWs.loop; simp
+
+@[simp]
+theorem readNatNoWs_eq_size (arr : ByteArray)
+    : readNatNoWs (α := α) arr arr.size.toUSize = (0, arr.size.toUSize) := by
+  simp [readNatNoWs]
+
+private theorem readNatNoWs_loop_le_of_le {arr : ByteArray} {iter : USize}
+    : iter ≤ arr.size.toUSize → ∀ (acc : α), (readNatNoWs.loop arr iter acc).2 ≤ arr.size.toUSize := by
+  intro hi acc
+  rcases USize.lt_or_eq_of_le hi with (h | h)
+  · unfold readNatNoWs.loop
+    simp [h]
+    split
+    · apply readNatNoWs_loop_le_of_le (USize.succ_le_of_lt h)
+    · split
+      · exact hi
+      · apply USize.le_refl
+  · simp [h]
+termination_by arr.size.toUSize - iter
+decreasing_by
+  simp
+  apply USize.lt_iff_toNat_lt.mp
+  apply USize.sub_lt_sub_of_lt_of_le
+  apply USize.lt_succ_of_lt (by assumption)
+  apply USize.succ_le_of_lt (by assumption)
+
+theorem readNatNoWs_le_of_le {arr : ByteArray} {iter : USize}
+    : iter ≤ arr.size.toUSize → (readNatNoWs (α := α) arr iter).2 ≤ arr.size.toUSize := by
+  intro hi
+  unfold readNatNoWs
+  simp
+  split
+  · apply readNatNoWs_loop_le_of_le hi
+  · exact hi
+
+@[simp]
+theorem iter_le_readNat (arr : ByteArray) (iter : USize)
+    : iter ≤ (readNat (α := α) arr iter).2 := by
+  unfold readNat
+  simp
+  have h₁ := iter_le_ws arr iter
+  have h₂ := iter_le_readNatNoWs (α := α) arr (ws arr iter)
+  exact USize.le_trans h₁ h₂
+
+@[simp]
+theorem readNat_loop_eq_size (arr : ByteArray)
+    : readNat arr arr.size.toUSize = (0, arr.size.toUSize) := by
+  simp [readNat]
+
+theorem readNat_iter_le_of_le {arr : ByteArray} {iter : USize}
+    : iter ≤ arr.size.toUSize → (readNat (α := α) arr iter).2 ≤ arr.size.toUSize := by
+  intro hi
+  simp [readNat]
+  exact readNatNoWs_le_of_le <| ws_le_of_le hi
+
+@[simp]
+theorem iter_le_readInt_iter (arr : ByteArray) (iter : USize)
+    : iter ≤ (readInt (α := α) arr iter).2 := by
+  unfold readInt
+  simp
+  have h₁ := iter_le_ws arr iter
+  split
+  · rename_i hp
+    have : peek arr (ws arr iter) ≠ UInt8.EOF := by simp [hp]
+    replace := iter_lt_of_peek_ne_EOF this
+    simp
+    apply USize.le_trans h₁
+    apply USize.le_trans (USize.le_of_lt (USize.lt_succ_of_lt this))
+    apply iter_le_readNatNoWs
+    done
+  · simp
+    apply USize.le_trans h₁
+    apply iter_le_readNatNoWs
+
+@[simp]
+theorem readInt_eq_size (arr : ByteArray)
+    : readInt (α := α) arr arr.size.toUSize = (0, arr.size.toUSize) := by
+  simp [readInt]
+
+theorem readInt_iter_le_of_le {arr : ByteArray} {iter : USize}
+    : iter ≤ arr.size.toUSize → (readInt (α := α) arr iter).2 ≤ arr.size.toUSize := by
+  intro hi
+  simp [readInt]
+  split
+  <;> simp
+  · rename_i hp
+    have : peek arr (ws arr iter) ≠ UInt8.EOF := by simp [hp]
+    replace := iter_lt_of_peek_ne_EOF this
+    apply readNatNoWs_le_of_le
+    exact USize.succ_le_of_lt this
+  · exact readNatNoWs_le_of_le <| ws_le_of_le hi
+
+
+
+theorem iter_lt_readNat_of_ne_zero {arr : ByteArray} {iter : USize}
+    : (readNat (α := α) arr iter).1 ≠ 0 → iter < (readNat (α := α) arr iter).2 := by
+  unfold readNat
+  simp
+  intro h
+  apply USize.lt_of_le_of_lt <| iter_le_ws arr iter
+  apply iter_lt_readNatNoWs_of_ne_zero
+  exact h
+
+theorem iter_lt_readInt_iter_of_ne_zero {arr : ByteArray} {iter : USize}
+    : (readInt (α := α) arr iter).1 ≠ 0 → iter < (readInt (α := α) arr iter).2 := by
+  unfold readInt
+  simp
+  split
+  · rename_i hp
+    have : peek arr (ws arr iter) ≠ UInt8.EOF := by simp [hp]
+    replace := iter_lt_of_peek_ne_EOF this
+    simp at this
+    simp
+    intro h
+    apply USize.lt_of_le_of_lt (iter_le_ws arr iter)
+    apply USize.lt_trans (USize.lt_succ_of_lt this)
+    apply iter_lt_readNatNoWs_of_ne_zero
+    intro h_con
+    simp [h_con] at h
+  · simp
+    intro h
+    apply USize.lt_of_le_of_lt <| iter_le_ws arr iter
+    apply iter_lt_readNatNoWs_of_ne_zero
+    intro h_con
+    simp [h_con] at h
+
+end readNat /- section -/
+
+end ByteArray
