Experiments/SR/Data/ByteArray/Defs.lean
@@ -1,0 +1,344 @@
+/-
+Copyright (c) 2024 The Trestle Contributors.
+Released under the Apache License v2.0; see LICENSE for full text.
+
+Authors: Cayden Codel
+-/
+
+import Lean
+import Experiments.SR.Data.UInt.Basic
+import Experiments.SR.Data.UInt.Defs
+
+/-!
+
+A modification of `String.Iterator` on `ByteArray`s.
+It assumes that the string, represented as a `ByteArray` is in ASCII format.
+
+These functions are written with efficiency in mind.
+In general, these functions take in `ByteArray` and an iterator `iter`,
+but they only return an updated `iter`, since the array is not modified.
+In addition, the iterator is a `USize` as opposed to a `Nat`,
+since the length of the string (array) is assumed to fit in a `USize`.
+
+-/
+
+namespace ByteArray
+
+/--
+  Peeks at the character under the iterator.
+  Returns `UInt8.EOF` if the iterator is out of bounds.
+-/
+def peek (arr : ByteArray) (iter : USize) : UInt8 :=
+  if hi : iter < arr.usize then
+    arr.uget iter (USize.toNat_lt_of_lt_toUSize hi)
+  else
+    UInt8.EOF
+
+/-- A Lean version of `getc` from C/C++. An alias for `peek`. -/
+@[simp] abbrev getc := peek
+
+/--
+  Skips characters in `arr` meeting a predicate `pred`, starting from `iter`.
+  On return, `iter` points to the first character that does NOT meet `pred`.
+
+  If `iter` is out of bounds, `iter` is returned.
+-/
+@[specialize]
+def skip (arr : ByteArray) (iter : USize) (pred : UInt8 → Bool) : USize :=
+  if hi : iter < arr.usize then
+    let ch := arr.uget iter (USize.toNat_lt_of_lt_toUSize hi)
+    if pred ch then
+      skip arr (iter + 1) pred
+    else
+      iter
+  else
+    iter
+termination_by arr.usize - iter
+decreasing_by simp; apply USize.lt_iff_toNat_lt.mp; apply USize.sub_succ_lt_sub_of_lt; assumption
+
+/--
+  Moves the iterator forward until it points to the first non-whitespace character.
+-/
+@[extern "lean_byte_array_ws"]
+def ws (arr : @& ByteArray) (iter : USize) : USize :=
+  skip arr iter (·.isSpace)
+
+/--
+  Consumes a line until and including the first newline character `'\n'`.
+  Returns the updated iterator, which either points to just after the newline
+  character, or to the end of the array if no newline is found.
+-/
+@[extern "lean_byte_array_line"]
+def line (arr : ByteArray) (iter : USize) : USize :=
+  let iter := skip arr iter (! ·.isNewline)
+  if iter < arr.usize then
+    iter + 1
+  else
+    iter
+
+/--
+  Consumes the next token and any preceding whitespace.
+  On return, `iter` points to the first whitespace character after the
+  first contiguous sequence of non-whitespace characters,
+  or to the end of the array.
+-/
+@[extern "lean_byte_array_token"]
+def token (arr : ByteArray) (iter : USize) : USize :=
+  let iter := ws arr iter
+  skip arr iter (! ·.isSpace)
+
+@[extern "lean_byte_array_skip_nat_no_ws"]
+def skipNatNoWs (arr : @& ByteArray) (iter : USize) : USize :=
+  skip arr iter (·.isDigit)
+
+@[extern "lean_byte_array_skip_int_no_ws"]
+def skipIntNoWs (arr : @& ByteArray) (iter : USize) : USize :=
+  let ch := peek arr iter
+  if ch = Char.toUInt8 '-' then
+    skipNatNoWs arr (iter + 1)
+  else
+    skipNatNoWs arr iter
+
+def skipNat (arr : ByteArray) (iter : USize) : USize :=
+  let iter := ws arr iter
+  skipNatNoWs arr iter
+
+def skipInt (arr : ByteArray) (iter : USize) : USize :=
+  let iter := ws arr iter
+  skipIntNoWs arr iter
+
+/-! # readNat and readInt -/
+
+class ParseNumeric (α : Type u)
+  extends Add α, Zero α where
+  ofUInt8 : UInt8 → α
+  mulTen : α → α
+  toInt : α → Int
+  toInt_zero : toInt (0 : α) = 0
+
+attribute [simp] ParseNumeric.toInt_zero
+
+instance (α : Type u) [ParseNumeric α] : Inhabited α where
+  default := 0
+
+@[simp] theorem ParseNumeric.default_eq_zero (α : Type u) [ParseNumeric α] : (default : α) = 0 := rfl
+
+instance : ParseNumeric USize where
+  ofUInt8 := UInt8.digitToUSize
+  mulTen n := n * (10 : USize)
+  toInt n := Int.ofNat n.toNat
+  toInt_zero := rfl
+
+instance : ParseNumeric UInt16 where
+  ofUInt8 := UInt8.digitToUInt16
+  mulTen n := n * (10 : UInt16)
+  toInt n := Int.ofNat n.toNat
+  toInt_zero := rfl
+
+instance : ParseNumeric UInt32 where
+  ofUInt8 := UInt8.digitToUInt32
+  mulTen n := n * (10 : UInt32)
+  toInt n := Int.ofNat n.toNat
+  toInt_zero := rfl
+
+instance : ParseNumeric UInt64 where
+  ofUInt8 := UInt8.digitToUInt64
+  mulTen n := n * (10 : UInt64)
+  toInt n := Int.ofNat n.toNat
+  toInt_zero := rfl
+
+instance : ParseNumeric Nat where
+  ofUInt8 := UInt8.digitToNat
+  mulTen n := n * (10 : Nat)
+  toInt n := Int.ofNat n
+  toInt_zero := rfl
+
+/--
+  Reads a natural number from `arr` starting at `iter`. Parsing stops
+  at the first non-digit character, or when the end of the array is reached.
+
+  If the first character is not a digit, `0` is returned, and `iter` is unchanged.
+
+  The `ParseNumeric` type enables different fixed-width representations
+  to be parsed, which might be more efficient than `Nat`s.
+-/
+@[specialize]
+def readNatNoWs {α : Type u} [ParseNumeric α] (arr : ByteArray) (iter : USize) (acc : α := 0) : α × USize :=
+  if hi : iter < arr.usize then
+    let ch := arr.uget iter (USize.toNat_lt_of_lt_toUSize hi)
+    if ch.isDigit then
+      readNatNoWs arr (iter + 1) (ParseNumeric.mulTen acc + ParseNumeric.ofUInt8 ch)
+    else
+      (acc, iter)
+  else
+    (acc, iter)
+termination_by arr.usize - iter
+decreasing_by simp; apply USize.lt_iff_toNat_lt.mp; apply USize.sub_succ_lt_sub_of_lt; assumption
+
+/--
+  A wrapper for `readNatNoWs` that checks if the first character is a digit.
+  If not, or if the iterator is out of bounds, the function panics.
+-/
+@[specialize]
+def readNatNoWs! {α : Type u} [ParseNumeric α] (arr : ByteArray) (iter : USize) : α × USize :=
+  if iter < arr.usize then
+    let ch := peek arr iter
+    if ch.isDigit then
+      readNatNoWs arr iter 0
+    else
+      let n := panic! "Attempted to read a Nat, but the first character is not a digit: {Char.ofNat ch.toNat}"
+      (n, iter)
+  else
+    let n := panic! "Attempted to read a Nat, but the iterator is out of bounds"
+    (n, iter)
+
+@[specialize, inline, always_inline]
+def readNat {α : Type u} [ParseNumeric α] (arr : ByteArray) (iter : USize) : α × USize :=
+  let iter := ws arr iter
+  if iter < arr.usize then
+    readNatNoWs arr iter 0
+  else
+    (0, iter)
+
+@[specialize, inline, always_inline]
+def readNat! {α : Type u} [ParseNumeric α] (arr : ByteArray) (iter : USize) : α × USize :=
+  let iter := ws arr iter
+  readNatNoWs! arr iter
+
+/--
+  Parses an integer using an internal accumulator type `α`.
+  Using a fixed-width type such as `UInt32` will be more efficient.
+-/
+@[specialize]
+def readInt (α : Type u) [ParseNumeric α] (arr : ByteArray) (iter : USize) : Int × USize :=
+  let iter := ws arr iter
+  let ch := peek arr iter
+  if ch = Char.toUInt8 '-' then
+    let (n, iter) := readNatNoWs (α := α) arr (iter + 1) 0
+    (-(ParseNumeric.toInt n), iter)
+  else if ch.isDigit then
+    let (n, iter) := readNatNoWs (α := α) arr iter 0
+    (ParseNumeric.toInt n, iter)
+  else
+    (0, iter)
+
+/--
+  A version of `readInt` that panics if the first character is not 0-9 or '-',
+  or if the iterator is out of bounds.
+-/
+@[specialize]
+def readInt! (α : Type u) [ParseNumeric α] (arr : ByteArray) (iter : USize) : Int × USize :=
+  let iter := ws arr iter
+  let ch := peek arr iter
+  if ch = Char.toUInt8 '-' then
+    let (n, iter) := readNatNoWs! (α := α) arr (iter + 1)
+    (-(ParseNumeric.toInt n), iter)
+  else if ch.isDigit then
+    let (n, iter) := readNatNoWs! (α := α) arr iter
+    (ParseNumeric.toInt n, iter)
+  else if ch = UInt8.EOF then
+    let n := panic! "Attempted to read an integer, but the iterator is out of bounds"
+    (n, iter)
+  else
+    let n := panic! s!"Attempted to read an integer, but the first character is not a digit or '-': {Char.ofNat ch.toNat}"
+    (n, iter)
+
+/-! # readUInt variants -/
+
+def readUInt32NoWs.loop (arr : ByteArray) (iter : USize) (acc : UInt32) : UInt32 :=
+  if hi : iter < arr.usize then
+    let ch := arr.uget iter (USize.toNat_lt_of_lt_toUSize hi)
+    if ch.isDigit then
+      readUInt32NoWs.loop arr (iter + 1) (acc * 10 + UInt8.digitToUInt32 ch)
+    else
+      acc
+  else
+    acc
+termination_by arr.usize - iter
+decreasing_by simp; apply USize.lt_iff_toNat_lt.mp; apply USize.sub_succ_lt_sub_of_lt; assumption
+
+/--
+  Reads a 32-bit unsigned integer from `arr` starting at `iter`, but doesn't
+  move the iterator.  Call `skipNat` after to move the iterator forward.
+-/
+@[extern "lean_byte_array_read_uint32_no_ws"]
+def readUInt32NoWs (arr : @& ByteArray) (iter : USize) : UInt32 :=
+  if iter < arr.usize then
+    let ch := peek arr iter
+    if ch.isDigit then
+      readUInt32NoWs.loop arr iter 0
+    else
+      panic! s!"Attempted to read a UInt32, but the first character is not a digit: {Char.ofNat ch.toNat}"
+  else
+    panic! "Attempted to read a UInt32, but the iterator is out of bounds"
+
+@[inline]
+def readUInt32 (arr : ByteArray) (iter : USize) : UInt32 :=
+  let iter := ws arr iter
+  readUInt32NoWs arr iter
+
+@[extern "lean_byte_array_read_int32_no_ws"]
+def readInt32NoWs (arr : @& ByteArray) (iter : USize) : Int :=
+  if iter < arr.usize then
+    let ch := peek arr iter
+    if ch = Char.toUInt8 '-' then
+      (-(Int.ofNat <| UInt32.toNat <| readUInt32NoWs arr (iter + 1)))
+    else
+      Int.ofNat <| UInt32.toNat <| readUInt32NoWs arr iter
+  else
+    panic! "Attempted to read an Int32, but the iterator is out of bounds"
+
+@[inline]
+def readInt32 (arr : ByteArray) (iter : USize) : Int :=
+  let iter := ws arr iter
+  readInt32NoWs arr iter
+
+def readUInt64NoWs.loop (arr : ByteArray) (iter : USize) (acc : UInt64) : UInt64 :=
+  if hi : iter < arr.usize then
+    let ch := arr.uget iter (USize.toNat_lt_of_lt_toUSize hi)
+    if ch.isDigit then
+      readUInt64NoWs.loop arr (iter + 1) (acc * 10 + UInt8.digitToUInt64 ch)
+    else
+      acc
+  else
+    acc
+termination_by arr.usize - iter
+decreasing_by simp; apply USize.lt_iff_toNat_lt.mp; apply USize.sub_succ_lt_sub_of_lt; assumption
+
+/--
+  Reads a 64-bit unsigned integer from `arr` starting at `iter`, but doesn't
+  move the iterator.  Call `skipNat` after to move the iterator forward.
+-/
+@[extern "lean_byte_array_read_uint64_no_ws"]
+def readUInt64NoWs (arr : @& ByteArray) (iter : USize) : UInt64 :=
+  if iter < arr.usize then
+    let ch := peek arr iter
+    if ch.isDigit then
+      readUInt64NoWs.loop arr iter 0
+    else
+      panic! s!"Attempted to read a UInt64, but the first character is not a digit: {Char.ofNat ch.toNat}"
+  else
+    panic! "Attempted to read a UInt64, but the iterator is out of bounds"
+
+@[inline]
+def readUInt64 (arr : ByteArray) (iter : USize) : UInt64 :=
+  let iter := ws arr iter
+  readUInt64NoWs arr iter
+
+@[extern "lean_byte_array_read_int64_no_ws"]
+def readInt64NoWs (arr : @& ByteArray) (iter : USize) : Int :=
+  if iter < arr.usize then
+    let ch := peek arr iter
+    if ch = Char.toUInt8 '-' then
+      (-(Int.ofNat <| UInt64.toNat <| readUInt64NoWs arr (iter + 1)))
+    else
+      Int.ofNat <| UInt64.toNat <| readUInt64NoWs arr iter
+  else
+    panic! "Attempted to read an Int64, but the iterator is out of bounds"
+
+@[inline]
+def readInt64 (arr : ByteArray) (iter : USize) : Int :=
+  let iter := ws arr iter
+  readInt64NoWs arr iter
+
+end ByteArray /- namespace -/
