Experiments/SR/Data/UInt/Defs.lean
@@ -1,0 +1,151 @@
+
+import Init.Data.UInt.Basic
+
+namespace UInt8
+
+def maxVal : UInt8 := ⟨UInt8.size - 1, by rw [size]; omega⟩
+
+abbrev EOF : UInt8 := maxVal
+
+@[extern "uint8_is_digit"]
+def isDigit (c : UInt8) : Bool :=
+     c == (Char.toUInt8 '0')
+  || c == (Char.toUInt8 '1')
+  || c == (Char.toUInt8 '2')
+  || c == (Char.toUInt8 '3')
+  || c == (Char.toUInt8 '4')
+  || c == (Char.toUInt8 '5')
+  || c == (Char.toUInt8 '6')
+  || c == (Char.toUInt8 '7')
+  || c == (Char.toUInt8 '8')
+  || c == (Char.toUInt8 '9')
+
+theorem ne_EOF_of_isDigit {c : UInt8} : isDigit c → c ≠ EOF := by
+  simp [isDigit]
+  rintro h rfl
+  contradiction
+
+@[extern "uint8_is_space"]
+def isSpace (c : UInt8) : Bool :=
+     c == (Char.toUInt8 ' ')
+  || c == (Char.toUInt8 '\t')
+  || c == (Char.toUInt8 '\n')
+  || c == 11         -- '\v'
+  || c == 12         -- '\f'
+  || c == (Char.toUInt8 '\r')
+
+theorem ne_EOF_of_isSpace {c : UInt8} : isSpace c → c ≠ EOF := by
+  simp [isSpace]
+  rintro h rfl
+  contradiction
+
+@[inline, always_inline]
+def isNewline (c : UInt8) : Bool :=
+  c == (Char.toUInt8 '\n')
+
+/--
+  Converts an ASCII digit character to its numeric value.
+  If `c` is not an ASCII digit, the result is unspecified.
+
+  The designers of the ASCII codes were clever: the characters 0-9 start at
+  decimal value 48, which has binary 0b00001100. This means that if we mask
+  by 15 (0b11110000), we can get the numbers directly.
+-/
+@[inline, always_inline]
+private def asciiDigitToDigit (c : UInt8) : UInt8 :=
+  c &&& 15    -- 0b1111
+
+@[inline, always_inline]
+def digitToNat (c : UInt8) : Nat :=
+  (asciiDigitToDigit c).toNat
+
+@[inline, always_inline]
+def digitToInt (c : UInt8) : Int :=
+  Int.ofNat <| c.digitToNat
+
+@[inline, always_inline]
+def digitToUSize (c : UInt8) : USize :=
+  UInt8.toUSize <| asciiDigitToDigit c
+
+@[inline, always_inline]
+def digitToUInt16 (c : UInt8) : UInt16 :=
+  UInt8.toUInt16 <| asciiDigitToDigit c
+
+@[inline, always_inline]
+def digitToUInt32 (c : UInt8) : UInt32 :=
+  UInt8.toUInt32 <| asciiDigitToDigit c
+
+@[inline, always_inline]
+def digitToUInt64 (c : UInt8) : UInt64 :=
+  UInt8.toUInt64 <| asciiDigitToDigit c
+
+end UInt8
+
+namespace UInt32
+
+def maxVal : UInt32 := ⟨UInt32.size - 1, by rw [size]; omega⟩
+def EOF : UInt32 := maxVal
+
+@[extern "uint32_is_digit"]
+def isDigit (c : UInt32) : Bool :=
+     c == (UInt8.toUInt32 <| Char.toUInt8 '0')
+  || c == (UInt8.toUInt32 <| Char.toUInt8 '1')
+  || c == (UInt8.toUInt32 <| Char.toUInt8 '2')
+  || c == (UInt8.toUInt32 <| Char.toUInt8 '3')
+  || c == (UInt8.toUInt32 <| Char.toUInt8 '4')
+  || c == (UInt8.toUInt32 <| Char.toUInt8 '5')
+  || c == (UInt8.toUInt32 <| Char.toUInt8 '6')
+  || c == (UInt8.toUInt32 <| Char.toUInt8 '7')
+  || c == (UInt8.toUInt32 <| Char.toUInt8 '8')
+  || c == (UInt8.toUInt32 <| Char.toUInt8 '9')
+
+@[extern "uint32_is_space"]
+def isSpace (c : UInt32) : Bool :=
+     c == (UInt8.toUInt32 <| Char.toUInt8 ' ')
+  || c == (UInt8.toUInt32 <| Char.toUInt8 '\t')
+  || c == (UInt8.toUInt32 <| Char.toUInt8 '\n')
+  || c == 11                           -- '\v'
+  || c == 12                           -- '\f'
+  || c == (UInt8.toUInt32 <| Char.toUInt8 '\r')
+
+def numDigits (x : UInt32) : UInt32 :=
+  if x < 10 then 1
+  else if x < 100 then 2
+  else if x < 1000 then 3
+  else if x < 10000 then 4
+  else if x < 100000 then 5
+  else if x < 1000000 then 6
+  else if x < 10000000 then 7
+  else if x < 100000000 then 8
+  else if x < 1000000000 then 9
+  else 10
+
+end UInt32 /- namespace -/
+
+export UInt32 (EOF)
+
+namespace UInt64
+
+def numDigits (x : UInt64) : UInt64 :=
+  if x < 10 then 1
+  else if x < 100 then 2
+  else if x < 1000 then 3
+  else if x < 10000 then 4
+  else if x < 100000 then 5
+  else if x < 1000000 then 6
+  else if x < 10000000 then 7
+  else if x < 100000000 then 8
+  else if x < 1000000000 then 9
+  else if x < 10000000000 then 10
+  else if x < 100000000000 then 11
+  else if x < 1000000000000 then 12
+  else if x < 10000000000000 then 13
+  else if x < 100000000000000 then 14
+  else if x < 1000000000000000 then 15
+  else if x < 10000000000000000 then 16
+  else if x < 100000000000000000 then 17
+  else if x < 1000000000000000000 then 18
+  else if x < 10000000000000000000 then 19
+  else 20
+
+end UInt64 /- namespace -/
