Experiments/SR/Parsing/SRParser.lean
@@ -6,7 +6,8 @@ Authors: Cayden Codel
 -/
 
 import Experiments.SR.Parsing.Defs
-import Experiments.SR.Data.AsciiIterator
+import Experiments.SR.Data.ByteArray.Defs
+import Experiments.SR.Data.ByteArray.Basic
 
 /-!
 
@@ -18,112 +19,198 @@ namespace Trestle
 
 namespace SRParser
 
-open Parsing
+open Parsing ByteArray
 
-variable {CNF : Type _} [Formula CNF] [Inhabited CNF]
+variable {CNF : Type _} [Formula CNF]
 
-partial def consumeCommentLines (arr : ByteArray') (iter : USize) : Except Unit USize :=
-  let c := ByteArray.peekc arr iter
-  if c = UInt8.EOF then .error () else
+def consumeCommentLines (arr : ByteArray) (iter : USize) : USize :=
+  let c : UInt8 := peek arr iter
   if c = 'c'.toUInt8 then
-    let rec loop (iter : USize) : Except Unit USize :=
-      let c := ByteArray.peekc arr iter
-      if c = UInt8.EOF then .error () else
-      if c = '\n'.toUInt8 then
-        .ok (iter+1)
-      else
-        loop (iter+1)
-    do
-      let iter ← loop iter
-      consumeCommentLines arr iter
+    consumeCommentLines arr <| line arr (iter + 1)
   else
-    .ok iter
+    iter
+termination_by arr.size.toUSize - iter
+decreasing_by
+  simp
+  rw [← USize.lt_iff_toNat_lt]
+  apply USize.sub_lt_sub_of_lt_of_le
+  <;> rename_i h
+  · have : c ≠ UInt8.EOF := by simp [h]; trivial
+    replace := iter_lt_of_peek_ne_EOF this
+    have h₁ := iter_le_line arr (iter + 1)
+    exact USize.lt_of_lt_of_le (USize.lt_succ_of_lt this) h₁
+  · apply line_le_of_le
+    have : c ≠ UInt8.EOF := by simp [h]; trivial
+    exact USize.succ_le_of_lt <| iter_lt_of_peek_ne_EOF this
 
+/-! # parseClause -/
 
+/--
+  Parses a clause from the array `arr` starting at `iter`.
+-/
 @[specialize]
-def parseClause (maxVar : Nat) (F : CNF) (arr : ByteArray') (iter : USize) : Except Unit (CNF × USize) := do
-  let size := arr.val.size.toUSize
-  let rec loop (F : CNF) (iter : USize) : Except Unit (CNF × USize) :=
-    if hi : iter < size then
-      let ⟨atom, iter'⟩ := ByteArray.readInt arr iter
-
-      if h_atom : atom = 0 then
-        .ok (Formula.commitClause F, iter')
+def parseClause (F : CNF) (arr : ByteArray) (maxVar : Nat) (iter : USize) : CNF × USize :=
+  if _ : iter < arr.size.toUSize then
+    match h_atom : ByteArray.readInt32 arr iter with
+    | atom =>
+    match h_iter' : ByteArray.skipInt arr iter with
+    | iter' =>
+    if h : atom = 0 then
+      (Formula.commitClause F, iter')
+    else
+      -- Out of bounds variable
+      if atom.natAbs > maxVar then
+        let F' : CNF := panic! s!"Variable {atom.natAbs} in clause {Formula.size F + 1} exceeds maximum variable {maxVar}"
+        (F', arr.size.toUSize)
       else
-        if atom.natAbs > maxVar then
-          -- Out of bounds variable
-          .error ()
-        else
-          have : (arr.val.size.toUSize - iter').toNat < (arr.val.size.toUSize - iter).toNat := by
-            have := ByteArray.readInt_iter_gt hi
-            sorry
-            done
-          loop (Formula.addLiteral F ⟨atom, h_atom⟩) iter'
-    else
-      .error ()
-  termination_by arr.val.size.toUSize - iter
+        parseClause (Formula.addLiteral F ⟨atom, by simp [h]⟩) arr maxVar iter'
+  else
+    (F, iter)
+termination_by arr.size.toUSize - iter
+decreasing_by
+  subst h_iter' h_atom
+  simp
+  apply USize.lt_iff_toNat_lt.mp
+  apply USize.sub_lt_sub_of_lt_of_le
+  · exact iter_lt_skipInt_of_readInt32 h
+  · apply skipInt_le_of_le
+    exact USize.le_of_lt (by assumption)
 
-  loop F iter
+-- @[simp]
+-- private theorem iter_le_parseClause_iter (F : CNF) (arr : ByteArray) (iter : USize) (maxVar : Nat)
+--     : iter ≤ (parseClause F arr maxVar iter).2 := by
+--   unfold parseClause
+--   stop
+--   simp
+--   split
+--   · rename_i hi
+--     split
+--     · simp
+--     · split
+--       · simp
+--         apply USize.le_of_lt (by assumption)
+--       · apply USize.le_trans <| iter_le_readInt_iter (α := UInt32) (arr := arr) (iter := iter)
+--         apply iter_le_parseClause_loop_iter
+--   · simp
+-- termination_by arr.size.toUSize - iter
+-- decreasing_by
+--   stop
+--   simp
+--   rw [← USize.lt_iff_toNat_lt]
+--   apply USize.sub_lt_sub_of_lt_of_le
+--   · apply iter_lt_readInt_iter_of_ne_zero (by assumption)
+--   · apply readInt_iter_le_of_le
+--     apply USize.le_of_lt (by assumption)
 
---@[inline, always_inline, specialize]
+-- private theorem parseClause_loop_iter_le_of_le (F : CNF) (arr : ByteArray) (iter : USize) (maxVar : Nat)
+--     : iter ≤ arr.size.toUSize → (parseClause F arr maxVar iter).2 ≤ arr.size.toUSize := by
+--   intro hi
+--   stop
+--   unfold parseClause.loop
+--   simp
+--   split
+--   · rename_i hi_lt
+--     split
+--     · simp
+--       exact readInt_iter_le_of_le hi
+--     · rename_i h_int
+--       split
+--       · simp
+--       · apply parseClause_loop_iter_le_of_le
+--         exact readInt_iter_le_of_le hi
+--   · exact USize.le_iff_toBitVec_le.mpr hi
+-- termination_by arr.size.toUSize - iter
+-- decreasing_by
+--   simp
+--   stop
+--   rw [← USize.lt_iff_toNat_lt]
+--   apply USize.sub_lt_sub_of_lt_of_le
+--   · apply iter_lt_readInt_iter_of_ne_zero (by assumption)
+--   · apply readInt_iter_le_of_le
+--     apply USize.le_of_lt (by assumption)
+
+-- theorem parseClause_iter_le_of_le (F : CNF) (arr : ByteArray) (iter : USize) (maxVar : Nat)
+--     : iter ≤ arr.size.toUSize → (parseClause F arr iter maxVar).2 ≤ arr.size.toUSize := by
+--   intro hi
+--   unfold parseClause
+--   simp
+--   apply parseClause_loop_iter_le_of_le
+--   exact USize.le_iff_toBitVec_le.mpr hi
+
+/-! # parseClauses -/
+
 @[specialize]
-partial def parseClauses (nvars ncls : Nat) (F : CNF) (arr : ByteArray') (iter : USize) : Except String CNF :=
-  let size := arr.val.size.toUSize
+partial def parseClauses (F : CNF) (arr : ByteArray) (iter : USize) (nVars nClauses : Nat) : Except String CNF := do
+  let size := arr.size.toUSize
   let rec loop (F : CNF) (iter : USize) : Except String (CNF × USize) :=
-    let iter := ByteArray.ws arr iter
-    if _ : iter < size then
-      match parseClause nvars F arr iter with
-      | .error _ => .error "Clause parsing error"
-      | .ok ⟨F, iter⟩ => loop F iter
+    have : size = arr.size.toUSize := rfl
+    let iter₂ := ws arr iter
+    if _ : iter₂ < size then
+      --let prevSize := Formula.size F
+      match _ : parseClause F arr nVars iter₂ with
+      | (F', iter₃) =>
+      -- if Formula.uncommittedSize F' != 0 || Formula.size F' = prevSize then
+      --   .error s!"Formula clause {Formula.size F' + 1} contained a parsing error"
+      -- else if iter₃ = iter₂ then
+      --   -- TODO(CC): Remove this branch by adding a theorem on `parseClause` that the iteraor *will* move forward
+      --   .error s!"Iterator did not advance forward in formula clause {Formula.size F' + 1}"
+      -- else
+        loop F' iter₃
     else
-      .ok (F, iter)
+      .ok (F, iter₂)
+  -- termination_by arr.size.toUSize - iter
+  -- decreasing_by
+  --   simp_wf
+  --   rw [← USize.lt_iff_toNat_lt]
+  --   rename_i hp _ h_ne
+  --   apply USize.sub_lt_sub_of_lt_of_le
+  --   · have := iter_le_parseClause_iter F arr iter₂ nVars
+  --     simp [hp] at this
+  --     exact USize.lt_of_le_of_ne this (Ne.symm h_ne)
+  --   · have := parseClause_iter_le_of_le F arr iter nVars
+  --     simp [hp] at this
+  --     exact this <| USize.le_of_lt (by assumption)
 
-  match loop F iter with
-  | .ok (F, _) =>
-    if Formula.size F != ncls then
-      throw s!"Expected {ncls} clauses, but found {Formula.size F}"
-    else
-      .ok F
-  | .error str => throw str
+  let (F, _) ← loop F iter
+  if Formula.size F != nClauses then
+    throw s!"Expected {nClauses} clauses, but parsed {Formula.size F}"
+  else
+    .ok F
 
---@[inline]
-def parseHeader (arr : ByteArray') (iter : USize) : Except String (Nat × Nat × USize) := do
-  let iter ← consumeCommentLines arr iter |>.mapError fun () => "Empty file?"
+def parseHeader (arr : ByteArray) (iter : USize) : Except String (Nat × Nat × USize) := do
+  let iter := consumeCommentLines arr iter
 
   -- Assumes that the first two non-whitespace tokens are "p" and "cnf"
-  let iter := ByteArray.skip arr iter
-  let iter := ByteArray.skip arr iter
+  let iter := token arr iter
+  let iter := token arr iter
 
   -- Now parse two nats
-  let ⟨nVars, iter⟩ := ByteArray.readNat arr iter
-  let ⟨nCls, iter⟩ := ByteArray.readNat arr iter
+  let ⟨nVars, iter⟩    := readNat arr iter
+  let ⟨nClauses, iter⟩ := readNat arr iter
 
-  if nVars = 0 || nCls = 0 || iter >= arr.val.size.toUSize then
-    throw s!"Invalid header: {nVars}, {nCls}, or iter out of bounds"
+  if nVars = 0 then
+    throw s!"Invalid cnf header: The number of variables was 0"
+  else if nClauses = 0 then
+    throw s!"Invalid cnf header: The number of clauses was 0"
   else
-    .ok (nVars, nCls, iter)
+    .ok (nVars, nClauses, iter)
 
 @[specialize]
-def parseFormula (arr : ByteArray') (F : CNF) : Except String (CNF × Nat) :=
-  match parseHeader arr 0 with
-  | .error str => throw str
-  | .ok (nvars, ncls, iter) =>
-    dbgTrace s!"Parsing formula with {nvars} variables, {ncls} clauses" fun () =>
-    match parseClauses nvars ncls F arr iter with
-    | .ok F =>
-      dbgTrace s!"Parsed formula" fun () =>
-        .ok (F, nvars)
-    | .error str => throw str
+def parseCnf (arr : ByteArray) (F : CNF) : Except String (CNF × Nat) := do
+  let ⟨nVars, nClauses, iter⟩ ← parseHeader arr 0
+  dbgTrace s!"c Parsing formula with {nVars} variables, {nClauses} clauses" fun () => do
+  let F ← parseClauses F arr iter nVars nClauses
+  return (F, nVars)
 
 -- CC: Because the parse line is called at top-level, it's okay for this to be Except.
 -- Returns the line id, the updated formula (with the candidate clause loaded), and the line
 @[specialize]
-partial def parseLSRAdditionLine (F : CNF) (arr : ByteArray') (iter : USize) : Except String (USize × CNF × SRAdditionLine) :=
+partial def parseLSRAdditionLine (F : CNF) (arr : ByteArray) (iter : USize) : Except String (USize × CNF × SRAdditionLine) :=
   -- Assume that `iter` is after the line ID, and that there is no `'d'`.
   -- Parse the first integer to get the pivot (or 0 for the empty clause)
-  let size := arr.val.size.toUSize
+  let size := arr.size.toUSize
   let line := SRAdditionLine.new
-  let ⟨pivot, iter⟩ := ByteArray.readInt arr iter
+  let ⟨pivot, iter⟩ := ByteArray.readInt (α := UInt32) arr iter
   let st :=
     if hp : pivot = 0 then
       ParsingState.mk .upHints F line
@@ -132,30 +219,57 @@ partial def parseLSRAdditionLine (F : CNF) (arr : ByteArray') (iter : USize) : E
 
   let rec loop (st : ParsingState CNF) (iter : USize) : Except String (USize × CNF × SRAdditionLine) :=
     if _ : iter < size then
-      let ⟨atom, iter⟩ := ByteArray.readInt arr iter
+      -- match _ : ByteArray.readInt64' arr iter with
+      -- | ⟨atom, iter'⟩ =>
+      let atom := ByteArray.readInt64 arr iter
+      let iter' := ByteArray.skipInt arr iter
       have ⟨mode, F, line⟩ := processSRAtom atom pivot st
       match mode with
       | .err str => throw str
-      | .lineDone => .ok (iter, F, line)
-      | _ => loop ⟨mode, F, line⟩ iter
+      | .lineDone => .ok (iter', F, line)
+      | _ => loop ⟨mode, F, line⟩ iter'
     else
       throw "Line ended early"
+  -- termination_by arr.size.toUSize - iter
+  -- decreasing_by
+  --   simp
+  --   rw [← USize.lt_iff_toNat_lt]
+  --   sorry
 
   loop st iter
 
 @[specialize]
-partial def parseDeletionLine (arr : ByteArray') (iter : USize) : Except String (Array Nat × USize) :=
+partial def parseDeletionLine (arr : ByteArray) (iter : USize) : Except String (Array Nat × USize) :=
   let iter := ByteArray.ws arr iter
-  let size := arr.val.size.toUSize
+  let size := arr.size.toUSize
 
   let rec loop (acc : Array Nat) (iter : USize) : Except String (Array Nat × USize) :=
+    have : size = arr.size.toUSize := rfl
     if _ : iter < size then
-      let ⟨atom, iter⟩ := ByteArray.readNat arr iter
+      let atom := ByteArray.readInt64 arr iter
+      let iter' := ByteArray.skipInt arr iter
       if atom = 0 then
-        .ok ⟨acc, iter⟩
+        .ok ⟨acc, iter'⟩
       else
-        loop (acc.push (atom - 1)) iter
+        loop (acc.push (atom - 1).toNat) iter'
     else
       throw "Line ended early"
+  -- termination_by arr.size.toUSize - iter
+  -- decreasing_by
+  --   simp
+  --   rw [← USize.lt_iff_toNat_lt]
+  --   rename_i hi h_readNat h_ne
+  --   stop
+  --   simp at h_readNat
+  --   apply USize.sub_lt_sub_of_lt_of_le
+  --   · have : atom = (readNat arr iter).1 := by simp [h_readNat]
+  --     rw [this] at h_ne
+  --     have := iter_lt_readNat_of_ne_zero h_ne
+  --     simp [h_readNat] at this
+  --     exact this
+  --   · have : iter' = (readNat (α := UInt64) arr iter).2 := by simp [h_readNat]
+  --     rw [this]
+  --     apply readNat_iter_le_of_le
+  --     apply USize.le_of_lt hi
 
   loop #[] iter
