lakefile.lean
@@ -1,5 +1,5 @@
 import Lake
-open Lake DSL
+open System Lake DSL
 
 package «trestle»
 
@@ -7,6 +7,7 @@ package «trestle»
 lean_lib Trestle {
   globs := #[.andSubmodules `Trestle]
 }
+
 
 lean_lib Examples {
   globs := #[.submodules `Examples]
@@ -21,8 +22,43 @@ lean_exe keller {
   --moreLeancArgs := #["-UNDEBUG", "-Og", "-ggdb", "-g3", "-fno-omit-frame-pointer"]
 }
 
+-- lean_lib ByteArrayFFI {
+--   globs := #[.submodules `Experiments.SR.Data.]
+-- }
+
+input_file byte_array_ffi_defs.c where
+  path := "Experiments" / "SR" / "Data" / "ByteArray" / "FFI" / "byte_array_ffi_defs.c"
+  text := true
+
+input_file uint_ffi_defs.c where
+  path := "Experiments" / "SR" / "Data" / "UInt" / "FFI" / "uint_ffi_defs.c"
+  text := true
+
+target byte_array_ffi_defs.o pkg : FilePath := do
+  let srcJob ← byte_array_ffi_defs.c.fetch
+  let oFile := pkg.buildDir / "c" / "byte_array_ffi_defs.o"
+  let weakArgs := #["-I", (← getLeanIncludeDir).toString]
+  buildO oFile srcJob weakArgs #["-fPIC"] "cc" getLeanTrace
+
+target uint_ffi_defs.o pkg : FilePath := do
+  let srcJob ← uint_ffi_defs.c.fetch
+  let oFile := pkg.buildDir / "c" / "uint_ffi_defs.o"
+  let weakArgs := #["-I", (← getLeanIncludeDir).toString]
+  buildO oFile srcJob weakArgs #["-fPIC"] "cc" getLeanTrace
+
+target libleanffi_static pkg : FilePath := do
+  let ba_ffiO ← byte_array_ffi_defs.o.fetch
+  let uint_ffiO ← uint_ffi_defs.o.fetch
+  let name := nameToStaticLib "leanffi"
+  buildStaticLib (pkg.staticLibDir / name) #[ba_ffiO, uint_ffiO]
+
 lean_exe srcheck {
   root := `Experiments.SR.Main
+  moreLinkObjs := #[libleanffi_static]
+}
+
+lean_exe test {
+  root := `Test
 }
 
 require mathlib from git "https://github.com/leanprover-community/mathlib4" @ "v4.28.0"
